

## 1.1 Vector Spaces

Why do we bother with a list of eight axioms? To a student first encountering Linear Algebra, this can feel like a bureaucratic exercise in “checking boxes.” However, there is a profound beauty hidden in this formality.

In our preliminary chapter, we saw three very different worlds: the world of geometric arrows ( $\mathbb{R}^n$ ), the world of functions ( $F[x]$ ), and the world of matrices ( $M_{m \times n}$ ). On the surface, an arrow is not a polynomial, and a polynomial is not a matrix. But if you squint, they all behave the same: you can add them, and you can scale them.

By defining a **Vector Space** through these axioms, we are choosing to ignore what the objects *are* and focus entirely on how they *act*. If we prove a theorem using only these eight axioms, that theorem becomes a “universal law” that applies to arrows, functions, and matrices all at once. This is the power of abstraction: solve the problem once, and you solve it for every universe that obeys these rules.

**Definition 1.1.1** (Vector Space). A set  $V$  over a field  $F$  with two operations: addition  $+$  and scalar multiplication  $\cdot$

$$+ : V \times V \rightarrow V, \quad \cdot : F \times V \rightarrow V$$

such that satisfy the following axioms for all  $\mathbf{v}_1, \mathbf{v}_2, \mathbf{v}_3 \in V$  and  $\alpha, \beta \in F$ :

$$(VS1) \quad \mathbf{v}_1 + \mathbf{v}_2 = \mathbf{v}_2 + \mathbf{v}_1$$

$$(VS2) \quad (\mathbf{v}_1 + \mathbf{v}_2) + \mathbf{v}_3 = \mathbf{v}_1 + (\mathbf{v}_2 + \mathbf{v}_3)$$

$$(VS3) \quad \text{There exists } \mathbf{0} \in V \text{ such that } \mathbf{v}_1 + \mathbf{0} = \mathbf{v}_1$$

$$(VS4) \quad \text{There exists } \mathbf{v}'_1 \in V \text{ such that } \mathbf{v}_1 + \mathbf{v}'_1 = \mathbf{0}$$

$$(VS5) \quad \alpha(\mathbf{v}_1 + \mathbf{v}_2) = \alpha\mathbf{v}_1 + \alpha\mathbf{v}_2$$

$$(VS6) \quad (\alpha + \beta)\mathbf{v}_1 = \alpha\mathbf{v}_1 + \beta\mathbf{v}_1$$

$$(VS7) \quad \alpha(\beta\mathbf{v}_1) = (\alpha\beta)\mathbf{v}_1$$

$$(VS8) \quad 1\mathbf{v}_1 = \mathbf{v}_1$$

*Remark.* Instead of writing  $(V, +, \cdot)$  is a vector space over  $F$ , we usually simplify it to  $V$  is a vector space over  $F$ , or even just  $V$  is a vector space if the context is clear.

*Remark.* We sometimes will abuse the name and refer to  $\mathbf{0} = \mathbf{0}_V \in V$  as the “zero vector” of the vector space  $V$ . Readers should not confuse  $\mathbf{0}_V$  with the zero scalar  $0 = 0_F \in F$  from the field  $F$ .

**Example** (Examples of Vector Spaces).

1. Most defaultly,  $F^n$  with the usual operations of  $+$  and  $\cdot$  is a vector space over  $F$ .
2. Working with polynomials is common too:  $F[x]$  with the usual operations of  $+$  and  $\cdot$  is a vector space over  $F$ .
3. Let  $\mathcal{D}$  be any open interval. Let

$$C(\mathcal{D}) := \{f : \mathcal{D} \rightarrow \mathbb{R} : f \text{ is continuous}\}.$$

Then  $C(\mathcal{D})$  is a vector space over  $\mathbb{R}$ . The zero vector of this vector space is given by the zero polynomial ( $x \mapsto 0$ ).

4. Let  $F$  be any field and fix  $n \in \mathbb{N}$ . Then  $M_n(F)$  is a vector space over  $F$ .
5. The set  $V = \mathbb{R}_{>0}$  of positive real numbers forms a vector space over  $F = \mathbb{R}$  under the following operations: for  $x, y \in V$  and  $\alpha \in F$ , define

$$x \oplus y := xy, \quad \alpha \odot x := x^\alpha = e^{\alpha \log x}.$$

Under these operations, the zero vector is  $\mathbf{0} = 1$ , and the additive inverse of  $x$  is  $x^{-1}$ .

You can check if addition and scalar multiplication make sense and follow all axioms of vector spaces.

**Example** ( $\mathbb{Q}$  Adjoin  $\sqrt{2}$ ). We verify that  $\mathbb{Q}(\sqrt{2}) := \{a + b\sqrt{2} : a, b \in \mathbb{Q}\}$  is a vector space over  $\mathbb{Q}$  by checking all eight axioms. Let  $\mathbf{v}_1 = a_1 + b_1\sqrt{2}$ ,  $\mathbf{v}_2 = a_2 + b_2\sqrt{2}$ ,  $\mathbf{v}_3 = a_3 + b_3\sqrt{2} \in \mathbb{Q}(\sqrt{2})$  and  $\alpha, \beta \in \mathbb{Q}$ .

$$(\text{VS1}) \quad \mathbf{v}_1 + \mathbf{v}_2 = (a_1 + a_2) + (b_1 + b_2)\sqrt{2} = (a_2 + a_1) + (b_2 + b_1)\sqrt{2} = \mathbf{v}_2 + \mathbf{v}_1.$$

$$(\text{VS2}) \quad (\mathbf{v}_1 + \mathbf{v}_2) + \mathbf{v}_3 = (a_1 + a_2 + a_3) + (b_1 + b_2 + b_3)\sqrt{2} = \mathbf{v}_1 + (\mathbf{v}_2 + \mathbf{v}_3).$$

$$(\text{VS3}) \quad \text{The element } \mathbf{0} = 0 + 0\sqrt{2} = 0 \in \mathbb{Q}(\sqrt{2}) \text{ satisfies } \mathbf{v}_1 + \mathbf{0} = (a_1 + 0) + (b_1 + 0)\sqrt{2} = \mathbf{v}_1.$$

$$(\text{VS4}) \quad \text{For } \mathbf{v}_1 = a_1 + b_1\sqrt{2}, \text{ define } -\mathbf{v}_1 := (-a_1) + (-b_1)\sqrt{2} \in \mathbb{Q}(\sqrt{2}). \text{ Then } \mathbf{v}_1 + (-\mathbf{v}_1) = (a_1 - a_1) + (b_1 - b_1)\sqrt{2} = \mathbf{0}.$$

$$(\text{VS5}) \quad \alpha(\mathbf{v}_1 + \mathbf{v}_2) = \alpha(a_1 + a_2) + \alpha(b_1 + b_2)\sqrt{2} = (\alpha a_1 + \alpha a_2) + (\alpha b_1 + \alpha b_2)\sqrt{2} = \alpha \mathbf{v}_1 + \alpha \mathbf{v}_2.$$

$$(\text{VS6}) \quad (\alpha + \beta)\mathbf{v}_1 = (\alpha + \beta)a_1 + (\alpha + \beta)b_1\sqrt{2} = (\alpha a_1 + \beta a_1) + (\alpha b_1 + \beta b_1)\sqrt{2} = \alpha \mathbf{v}_1 + \beta \mathbf{v}_1.$$

$$(\text{VS7}) \quad \alpha(\beta \mathbf{v}_1) = \alpha(\beta a_1 + \beta b_1\sqrt{2}) = \alpha\beta a_1 + \alpha\beta b_1\sqrt{2} = (\alpha\beta)\mathbf{v}_1.$$

$$(\text{VS8}) \quad 1 \cdot \mathbf{v}_1 = 1 \cdot a_1 + 1 \cdot b_1\sqrt{2} = a_1 + b_1\sqrt{2} = \mathbf{v}_1.$$

Thus  $\mathbb{Q}(\sqrt{2})$  is a vector space over  $\mathbb{Q}$ .

**Definition 1.1.2** (Vectors and Scalars). Let  $V$  be a vector space over  $F$ . Then the elements of  $V$  are called **vectors**, and the elements of  $F$  are called **scalars**.

Additionally,  $\mathbf{0} \in V$  is called the **zero vector**, and  $(\mathbf{v}'_1)$  in **(VS4)** is called the **inverse element** of  $\mathbf{v}_1$ .

**Theorem 1.1.1 (Left Cancellation Law).** Let  $V$  be a vector space over  $F$ , let  $\mathbf{u}, \mathbf{v}_1, \mathbf{v}_2 \in V$ . If  $\mathbf{u} + \mathbf{v}_1 = \mathbf{u} + \mathbf{v}_2$ , then  $\mathbf{v}_1 = \mathbf{v}_2$ .

*Proof.* Let  $\mathbf{u}'$  be an inverse of  $\mathbf{u}$ .

$$\begin{aligned}
 \mathbf{u} + \mathbf{v}_1 &= \mathbf{u} + \mathbf{v}_2 && \text{(given)} \\
 \mathbf{u}' + (\mathbf{u} + \mathbf{v}_1) &= \mathbf{u}' + (\mathbf{u} + \mathbf{v}_2) && \text{(add } \mathbf{u}' \text{ to both sides)} \\
 (\mathbf{u}' + \mathbf{u}) + \mathbf{v}_1 &= (\mathbf{u}' + \mathbf{u}) + \mathbf{v}_2 && \text{(by VS2)} \\
 \mathbf{0} + \mathbf{v}_1 &= \mathbf{0} + \mathbf{v}_2 && \text{(by VS4)} \\
 \mathbf{v}_1 &= \mathbf{v}_2 && \text{(by VS3)}
 \end{aligned}$$

■

**Theorem 1.1.2 (Right Cancellation Law).** Let  $V$  be a vector space over  $F$ , let  $\mathbf{u}, \mathbf{v}_1, \mathbf{v}_2 \in V$ . If  $\mathbf{v}_1 + \mathbf{u} = \mathbf{v}_2 + \mathbf{u}$ , then  $\mathbf{v}_1 = \mathbf{v}_2$ .

*Proof.* Since we have  $\mathbf{u} + \mathbf{v}_1 = \mathbf{u} + \mathbf{v}_2 \implies \mathbf{v}_1 = \mathbf{v}_2$ , applying **(VS1)** to it gives  $\mathbf{v}_1 + \mathbf{u} = \mathbf{v}_2 + \mathbf{u} \implies \mathbf{v}_1 = \mathbf{v}_2$ . ■

**Theorem 1.1.3 (Zero Vector is Unique).** Let  $V$  be a vector space over  $F$ . The zero vector  $\mathbf{0} \in V$  is unique.

*Proof.* Suppose that there are two vectors  $\mathbf{0}_1, \mathbf{0}_2$ .

$$\begin{aligned}
 \mathbf{0}_1 + \mathbf{0}_2 &= \mathbf{0}_2 + \mathbf{0}_1 && \text{(by VS1)} \\
 \mathbf{0}_1 &= \mathbf{0}_2 && \text{(by VS3)}
 \end{aligned}$$

■

**Theorem 1.1.4 (Additive Inverse is Unique).** Let  $V$  be a vector space over  $F$ . Then for every  $\mathbf{v} \in V$ , its additive inverse described in **(VS4)**, which is  $\mathbf{v}'$ , is unique.

*Proof.* Let  $\mathbf{v}'_1, \mathbf{v}'_2$  both be inverses of  $\mathbf{v}$ . Then

$$\begin{aligned}
 \mathbf{v}'_1 &= \mathbf{v}'_1 + \mathbf{0} && \text{(by VS3)} \\
 &= \mathbf{v}'_1 + (\mathbf{v} + \mathbf{v}'_2) && \text{(by VS4)} \\
 &= (\mathbf{v}'_1 + \mathbf{v}) + \mathbf{v}'_2 && \text{(by VS2)} \\
 &= \mathbf{0} + \mathbf{v}'_2 && \text{(by VS4)} \\
 &= \mathbf{v}'_2 && \text{(by VS3)}
 \end{aligned}$$

**Definition 1.1.3** (Notation of Additive Inverse). The unique inverse of a vector  $\mathbf{v} \in V$ , for a vector space  $V$  over  $F$ , will be denoted as  $-\mathbf{v}$ . ■

**Theorem 1.1.5 (Zero Scalar Annihilates).** Let  $\mathbf{v} \in V$  for a vector space  $V$  over  $F$ . Then  $0 \cdot \mathbf{v} = \mathbf{0}$ .

*Proof.* Let  $\mathbf{w} = 0 \cdot \mathbf{v}$ . We show that  $\mathbf{w} = \mathbf{0}$ .

$$\begin{aligned}
 \mathbf{w} + \mathbf{w} &= 0 \cdot \mathbf{v} + 0 \cdot \mathbf{v} \\
 &= (0 + 0) \cdot \mathbf{v} && \text{(by VS6)} \\
 &= 0 \cdot \mathbf{v} && \text{(arithmetic in } F) \\
 &= \mathbf{w} \\
 (\mathbf{w} + \mathbf{w}) + (-\mathbf{w}) &= \mathbf{w} + (-\mathbf{w}) && \text{(add } -\mathbf{w} \text{ to both sides)} \\
 \mathbf{w} + (\mathbf{w} + (-\mathbf{w})) &= \mathbf{0} && \text{(by VS2, VS4)} \\
 \mathbf{w} + \mathbf{0} &= \mathbf{0} && \text{(by VS4)} \\
 \mathbf{w} &= \mathbf{0} && \text{(by VS3)}
 \end{aligned}$$

**Theorem 1.1.6 (Negation as Scalar Multiplication).** Let  $V$  be a vector space over  $F$  and  $\mathbf{v} \in V$  be any vector. Then  $-\mathbf{v} = (-1) \cdot \mathbf{v}$ .

*Proof.* We show that  $(-1) \cdot \mathbf{v}$  is an additive inverse of  $\mathbf{v}$ :

$$\begin{aligned}
 \mathbf{v} + (-1) \cdot \mathbf{v} &= 1 \cdot \mathbf{v} + (-1) \cdot \mathbf{v} && \text{(by VS8)} \\
 &= (1 + (-1)) \cdot \mathbf{v} && \text{(by VS6)} \\
 &= 0 \cdot \mathbf{v} && \text{(arithmetic in } F) \\
 &= \mathbf{0} && \text{(by @thm-zero-scalar-mult)}
 \end{aligned}$$

Since  $(-1) \cdot \mathbf{v}$  is an additive inverse of  $\mathbf{v}$ , by uniqueness we have  $-\mathbf{v} = (-1) \cdot \mathbf{v}$ . ■

**Theorem 1.1.7 (Negative Scalar Distribution).** Let  $V$  be a vector space over  $F$ . For any  $\alpha \in F$  and  $\mathbf{v} \in V$ , we have  $(-\alpha)\mathbf{v} = -(\alpha\mathbf{v})$ .

*Proof.* We show that  $(-\alpha)\mathbf{v}$  is an additive inverse of  $\alpha\mathbf{v}$ :

$$\begin{aligned}\alpha\mathbf{v} + (-\alpha)\mathbf{v} &= (\alpha + (-\alpha))\mathbf{v} && \text{(by VS6)} \\ &= 0 \cdot \mathbf{v} && \text{(arithmetic in } F) \\ &= \mathbf{0} && \text{(by @thm-zero-scalar-mult)}\end{aligned}$$

Since  $(-\alpha)\mathbf{v}$  is an additive inverse of  $\alpha\mathbf{v}$ , by uniqueness we have  $(-\alpha)\mathbf{v} = -(\alpha\mathbf{v})$ . ■

**Theorem 1.1.8 (Scalar Multiplication by Zero Vector).** Let  $V$  be a vector space over  $F$ . For any scalar  $\alpha \in F$ , we have  $\alpha\mathbf{0} = \mathbf{0}$ .

*Proof.* Let  $\mathbf{w} = \alpha\mathbf{0}$ . We show that  $\mathbf{w} = \mathbf{0}$ .

$$\begin{aligned}\mathbf{w} &= \alpha\mathbf{0} \\ &= \alpha(\mathbf{0} + \mathbf{0}) && \text{(by VS3)} \\ &= \alpha\mathbf{0} + \alpha\mathbf{0} && \text{(by VS5)} \\ &= \mathbf{w} + \mathbf{w} \\ \mathbf{w} + (-\mathbf{w}) &= (\mathbf{w} + \mathbf{w}) + (-\mathbf{w}) && \text{(add } -\mathbf{w} \text{ to both sides)} \\ \mathbf{0} &= \mathbf{w} + (\mathbf{w} + (-\mathbf{w})) && \text{(by VS4, VS2)} \\ \mathbf{0} &= \mathbf{w} + \mathbf{0} && \text{(by VS4)} \\ \mathbf{0} &= \mathbf{w} && \text{(by VS3)}\end{aligned}$$

■

**Theorem 1.1.9 (Zero Product Law).** Let  $V$  be a vector space over  $F$ ,  $\mathbf{v} \in V$ , and  $\alpha \in F$ . If  $\alpha\mathbf{v} = \mathbf{0}$ , then either  $\alpha = 0$  or  $\mathbf{v} = \mathbf{0}$ .

*Proof.* Suppose  $\alpha\mathbf{v} = \mathbf{0}$ . We consider two cases:

- **Case  $\alpha = 0$ :** Then the statement holds.
- **Case  $\alpha \neq 0$ :** Since  $F$  is a field,  $\alpha$  has a multiplicative inverse  $\alpha^{-1}$ .

$$\begin{aligned}\alpha\mathbf{v} &= \mathbf{0} && \text{(given)} \\ \alpha^{-1}(\alpha\mathbf{v}) &= \alpha^{-1}\mathbf{0} && \text{(multiply by } \alpha^{-1}) \\ (\alpha^{-1}\alpha)\mathbf{v} &= \mathbf{0} && \text{(by VS7 and previous Theorem)} \\ 1 \cdot \mathbf{v} &= \mathbf{0} && \text{(field inverse property)} \\ \mathbf{v} &= \mathbf{0} && \text{(by VS8)}\end{aligned}$$

Thus, if  $\alpha \neq 0$ , we must have  $\mathbf{v} = \mathbf{0}$ . ■